mark-and-sweep/spec/GC.Spec.ChunkedMajorGC.Reachability.fsti
@@ -135,6 +135,18 @@ val chunked_gray_black_reachable_init
           Seq.mem x roots))
       (ensures chunked_gray_black_reachable mh roots)
 
+val chunked_gray_black_reachable_intro
+  (mh: MH.major_heap)
+  (roots: Seq.seq obj_addr)
+  : Lemma
+      (requires
+        (forall (x: obj_addr).
+          ChunkedMajorGraph.chunked_major_vertex mh x /\
+          (BDefs.chunked_is_gray mh x \/
+          SweepDefs.chunked_is_black mh x) ==>
+          chunked_major_reachable_from_roots mh roots x))
+      (ensures chunked_gray_black_reachable mh roots)
+
 val chunked_gray_black_reachable_elim
   (mh: MH.major_heap)
   (roots: Seq.seq obj_addr)
